Improve the handling of lambdas in the semantics (#185)

Lampe/Lampe/SeparationLogic/State.lean
@@ -85,10 +85,10 @@ def State.valSingleton (r : Ref) (v : AnyValue p) : SLP (State p) :=
 notation:max "[ " l " ↦ " r " ]" => State.valSingleton l r
 
 @[reducible]
-def State.lmbSingleton (r : Ref) (v : Lambda (Tp.denote p)) : SLP (State p) :=
-  fun st => st.lambdas = Finmap.singleton r v
+def State.lmbSingleton  (v : Lambda (Tp.denote p)) (r : FuncRef v.argTps v.outTp) : SLP (State p) :=
+  fun st => ∃ rr, r = FuncRef.lambda rr ∧ st.lambdas = Finmap.singleton rr v
 
-notation:max "[λ " l " ↦ " r " ]" => State.lmbSingleton l r
+notation:max "[λ " l " ↦ " r " ]" => State.lmbSingleton r l
 
 @[simp]
 lemma State.union_parts_left :
